theories/prelude/elpi/derive/finset.v
@@ -1,0 +1,93 @@
+(*
+ * Copyright (c) 2023 BedRock Systems, Inc.
+ * This software is distributed under the terms of the BedRock Open-Source License.
+ * See the LICENSE-BedRock file in the repository root for details.
+ *)
+From elpi Require Import elpi.
+From elpi.apps Require Import derive.
+
+From bedrock.prelude.elpi Require Import prelude derive.plugins.
+
+(***************************************************
+ Finite Sets
+ - [[ #[only(finset)] derive VariantType ]]
+   Assembles pieces from finite.v to expose `to_N` and `of_N` functions on `VariantType`, together with laws.
+   The encoding into `N` is derived automatically from the order of constructors of `VariantType`.
+ ***************************************************)
+Elpi Db derive.finset.db lp:{{
+  namespace derive.finset {
+    pred mk-finite-prelim i:string.
+    mk-finite-prelim TypeName :- std.do! [
+      coq.locate TypeName GR,
+      %TODO: I'd like to be able to do a transparent ascription here, but
+      %it doesn't seem like coq-elpi supports this (the following gives opaque ascription):
+      %coq.locate-module-type "simple_finite_bitmask_type_intf" MTP,
+      coq.env.begin-module TypeName none,
+
+      coq.env.add-const "t" (global GR) _ @transparent! C,
+      Ty = global (const C),
+
+      %TODO: these names are couplings, so centralize the calculation of instance names
+      %across Deriving and here.
+      EqdecName is TypeName ^ "_eq_dec",
+      coq.locate EqdecName GrEqdec,
+      std.assert-ok! (coq.elaborate-skeleton {{ EqDecision lp:{{ Ty }} }} _ ETyEqdec) "mk-finite-prelim: failed to check eq_dec",
+      coq.env.add-const "t_eq_dec" (global GrEqdec) ETyEqdec @transparent! Ceq_dec,
+      @global! => coq.TC.declare-instance (const Ceq_dec) 0,
+
+      FinName is TypeName ^ "_finite",
+      coq.locate FinName GrFin,
+      std.assert-ok! (coq.elaborate-skeleton {{ Finite lp:{{ Ty }} }} _ ETyFin) "mk-finite-prelim: failed to check finite",
+      coq.env.add-const "t_finite" (global GrFin) ETyFin @transparent! Cfin,
+      @global! => coq.TC.declare-instance (const Cfin) 0,
+    ].
+
+    pred mk-simple-finite i:string.
+    mk-simple-finite TypeName :- std.do! [
+      mk-finite-prelim TypeName,
+      coq.env.include-module-type {coq.locate-module-type "finite_type_mixin"} coq.inline.default,
+      coq.env.end-module MP_,
+    ].
+
+    pred mk-finite i:string, i:string.
+    mk-finite TypeName ToN :- std.do! [
+      mk-finite-prelim TypeName,
+
+      coq.locate "t" GRTy,
+      Ty is global GRTy,
+      coq.locate ToN GRtoN,
+      coq.env.add-const "to_N" (global GRtoN) {{ lp:Ty -> N }} @transparent! CtoN_,
+
+      coq.env.include-module-type {coq.locate-module-type "finite_encoded_type_mixin"} coq.inline.default,
+      coq.env.end-module MP_,
+    ].
+  }
+}}.
+
+Elpi Accumulate derive Db derive.finset.db.
+Elpi Accumulate derive lp:{{
+  namespace derive.finset {
+    pred main i:gref, i:string, o:list prop.
+    main TyGR Prefix Clauses :- std.do! [
+        remove-final-underscore Prefix Variant,
+      derive.finset.mk-simple-finite Variant,
+      Clauses = [finset-done TyGR],
+      std.forall Clauses (x\
+        coq.elpi.accumulate _ "derive.finbitset.db" (clause _ _ x)
+      ),
+    ].
+    main _ _ _ :- usage.
+
+    pred usage.
+    usage :- coq.error "Usage: derive.finset TyGR Prefix Clauses".
+  }
+
+  dep1 "finset" "finite". %finite implies eq_dec
+  derivation
+    (indt T) Prefix
+    (derive "finset"
+      (derive.finset.main (indt T) Prefix)
+      (finset-done (indt T))
+    ).
+}}.
+Elpi Typecheck derive.
